thys/Untyped_Lambda_Calculus/ILC_uniform.thy
@@ -18,7 +18,7 @@ by (auto intro!: reneqv.intros)
 lemma uniform_def2: "uniform e \<longleftrightarrow> (\<exists>e'. reneqv e' e)"
 unfolding uniform_def using reneweqv_sym by auto
 
-(* But to prove transitivity we will need inversion rules, which for the lambda cases 
+(* But to prove transitivity we will need inversion rules, which for the lambda case
 will require (1) the custom presSuper equivariance and (2) a custom supervariable-based injectivity for 
 lambda.  *)
 
@@ -37,10 +37,10 @@ lemma iLam_inject_super:
 assumes u: "uniform (iLam xs e)" and eq: "iLam xs e = iLam xs' e'" and super: "super xs" "super xs'"
 shows "\<exists>f. bij f \<and> |supp f| <o |UNIV::ivar set| \<and> presSuper f \<and> 
        id_on (ILC.FFVars (iLam xs e)) f \<and> id_on (- (dsset xs \<union> dsset xs')) f \<and> 
-           dsmap f xs = xs' \<and> rrename f e = e'"
+           dsmap f xs = xs' \<and> irrename f e = e'"
 proof-
   obtain f where f: "bij f \<and> |supp f| <o |UNIV::ivar set| \<and> id_on (FFVars (iLam xs e)) f \<and> 
-     dsmap f xs = xs' \<and> rrename f e = e'" using eq unfolding iLam_inject by auto
+     dsmap f xs = xs' \<and> irrename f e = e'" using eq unfolding iLam_inject by auto
   hence i: "inj_on f (dsset xs)" unfolding bij_def inj_on_def by auto
   define A where A: "A = FFVars (iLam xs e)"
   have 0: "|A| <o |UNIV::ivar set|" "finite (touchedSuper A)" "A \<inter> dsset xs = {}"
@@ -53,7 +53,7 @@ proof-
     subgoal using f by auto .
   show ?thesis using extend_super2[OF super 0] apply safe
   subgoal for g apply(rule exI[of _ g]) using f unfolding A eq_on_def id_on_def 
-    by (metis DiffI ILC.rrename_cong dstream.map_cong0 iterm.set(3)) .
+    by (metis DiffI ILC.irrename_cong dstream.map_cong0 iterm.set(3)) .
 qed
 
 lemma reneqv_iLam_casesL:
@@ -68,7 +68,7 @@ proof-
   
   obtain f where f: "bij f" "|supp f| <o |UNIV::ivar set|" "presSuper f" 
   "id_on (FFVars (iLam xsa ea)) f" "id_on (- (dsset xsa \<union> dsset xs)) f" 
-  and xsaa: "dsmap f xsa = xs" and e: "e = rrename f ea"
+  and xsaa: "dsmap f xsa = xs" and e: "e = irrename f ea"
   using iLam_inject_super[OF u il[symmetric] xsa xs] by auto
 
   have ff: "f ` (dsset xsa) = dsset xs" by (simp add: f(1) f(2) xsaa[symmetric])
@@ -81,14 +81,14 @@ proof-
   using super_disj[OF xs xsa] by auto
 
 
-  show ?thesis apply(rule exI[of _ "rrename f ea'"]) apply(intro conjI)
+  show ?thesis apply(rule exI[of _ "irrename f ea'"]) apply(intro conjI)
     subgoal unfolding ee' unfolding iLam_inject apply(rule exI[of _ f]) apply(intro conjI)
       subgoal by fact
       subgoal by fact
       subgoal apply simp using f(5) fv unfolding id_on_def by auto
       subgoal by fact
       subgoal .. . 
-    subgoal unfolding e using f(1) f(2) f(3) r rrename_reneqv by blast . 
+    subgoal unfolding e using f(1) f(2) f(3) r irrename_reneqv by blast . 
 qed
 
 lemma reneqv_iLam_casesR:
@@ -132,12 +132,12 @@ qed
 lemma uniform_def3: "uniform e \<longleftrightarrow> reneqv e e"
 using reneqv_trans reneweqv_sym uniform_def by blast
 
-corollary rrename_uniform:
+corollary irrename_uniform:
 assumes f: "bij f" "|supp f| <o |UNIV::ivar set|" "presSuper f"
 and r: "uniform (e::itrm)" 
-shows "uniform (rrename f e)"
+shows "uniform (irrename f e)"
 using assms unfolding uniform_def3 
-by (intro rrename_reneqv) auto
+by (intro irrename_reneqv) auto
 
 (* *)
 lemma reneqv_itvsubst:
